wip on continuations after call with Kenji and Exe

examples/dm4all/Cont2.fst
@@ -1,21 +1,25 @@
 module Cont2
 
-let repr (ans:Type) (a:Type) = (a -> ans) -> ans
+assume type ans
 
-let return (ans:Type) (a:Type) (x:a) = fun k -> k x
+let repr (a:Type) = (a -> ans) -> ans
 
-let bind (ans:Type) (a : Type) (b : Type)
-    (l : repr ans a) (f : a -> repr ans b) =
+let return (a:Type) (x:a) = fun k -> k x
+
+let bind (a : Type) (b : Type)
+    (l : repr a) (f : a -> repr b) =
     fun k -> l (fun x -> f x k)
 
-let wpty ans a = (a -> pure_wp ans) -> pure_wp ans
+let wpty a = (a -> pure_wp ans) -> pure_wp ans
 
-assume val x : ans:_ -> pure_wp ans
+let rel (#a : Type) (l : repr a) (w : wpty a) : Type =
+  forall (k : a -> ans) (p : ans -> Type). w (fun x q -> q (k x)) p == p (l k)
 
-//let interp (ans:Type) (a:Type) (l : repr ans a) : wpty ans a =
+let return_wp (a:Type) (x:a) : wpty a =
+  fun p -> p x
 
-let interp (ans:Type) (a:Type) (l : (a -> ans) -> ans) : (a -> pure_wp ans) -> pure_wp ans =
-  fun (kwp : a -> (ans -> Type) -> Type) (post : ans -> Type) -> post (l (fun (x:a) -> kwp x post))
+let bind_wp (_:range) (a b : Type) (m : wpty a) (f : a -> wpty b) : wpty b =
+  fun p -> m (fun x -> f x p)
 
 total
 reifiable
@@ -27,44 +31,39 @@ new_effect {
      ; return    = return
      ; bind      = bind
 
-     ; wp_type   = pure_wp
-     ; return_wp = pure_return
-     ; bind_wp   = pure_bind_wp
-
-     ; interp    = interp
-
-     (* ; choose    = choose *)
+     ; wp_type   = wpty
+     ; return_wp = return_wp
+     ; bind_wp   = bind_wp
 }
 
-let test1 () : CONT int (fun p -> p 5 /\ p 3) = 5
-let test2 () : CONT int (fun p -> p 5 /\ p 3) = 3
+let call_cc (#a:Type) (f : (a -> repr ans) -> repr ans) : repr a =
+  fun k -> f (fun (r:a) -> return _ (k r)) (fun x -> x)
 
-// Whoa! This used to succeed since the effect is marked as reifiable,
-// and Rel compares the representation types on each side for the
-// subtyping. and both are just `unit -> list a`. I changed it to check
-// the WPs via stronger-than instead of always unfolding.
-[@expect_failure]
-let test3 () : CONT int (fun p -> p 5 /\ p 3) = 4
+let call_cc_wp (#a:Type) (wpf : (a -> wpty ans) -> wpty ans) : wpty a =
+  fun (k : a -> pure_wp ans) (post : ans -> Type)
+       -> wpf (fun (r:a) (ww : ans -> pure_wp ans) -> pure_bind_wp range_0 _ _ (k r) ww) (fun x -> pure_return _ x) post
 
-effect Cont (a:Type) (pre:pure_pre) (post:pure_post' a pre) =
-        CONT a (fun (p:pure_post a) -> pre /\ (forall (pure_result:a). post pure_result ==> p pure_result))
+(* rel @ a -> repr ans *)
+let rel_1 (#a:Type) (f : a -> repr ans) (wpf : a -> wpty ans) : Type =
+  forall (x:a). rel (f x) (wpf x)
 
-effect ContTot (a:Type) = CONT a (pure_null_wp a)
+(* rel @ (a -> repr ans) -> ans *)
+let rel_2 (#a:Type) (f : (a -> repr ans) -> repr ans) (wpf : (a -> wpty ans) -> wpty ans) : Type =
+  forall g wpg. rel_1 g wpg ==> rel (f g) (wpf wpg)
 
-#set-options "--debug Continuations --debug_level SMTQuery"
+open FStar.Tactics
 
-let __em (#a:Type) : repr (c_or a (a -> Type)) =
-  fun (d : c_or a (a -> Type) -> Type) ->
-    let devil (x:a) : Type = d (Left x) in
-    d (Right devil)
+let call_cc_related #a (f : (a -> repr ans) -> repr ans) (wpf : (a -> wpty ans) -> wpty ans) :
+    Lemma (requires (rel_2 f wpf))
+          (ensures (rel (call_cc f) (call_cc_wp wpf)))
+          by (compute (); dump "Final")
+          = admit ()
 
-assume val em : (#a:Type) -> CONT (c_or a (a -> Type)) (fun p -> forall x. p x)
-// fails to typechecke due to universes..
-//let em #a = CONT?.reflect (__em #a)
+assume val callcc : #a:Type -> (#wpf:((a -> wpty ans) -> wpty ans)) ->
+                    (f : (#wpg:(a -> wpty ans) -> (x:a -> CONT ans (wpg x)) -> CONT ans (wpf wpg))) ->
+                    CONT a (call_cc_wp wpf)
 
-
-let callcc #a #b (f : a -> Type)
-
-
-[@expect_failure]
-let _ = assert False
+let em (#a:Type) : CONT (c_or a (a -> CONT ans (fun _ _ -> False))) (fun _ _ -> False) =
+  callcc #_ #(fun _ _ _ -> False)
+             (fun #_ (f : (x : c_or a (a -> CONT ans (fun _ _ -> False))) -> CONT ans (fun _ _ -> False)) ->
+                        f (Right (fun (x:a) -> f (Left x))))
